Inspect.lean
@@ -1,0 +1,12 @@
+import ITree.Basic
+import Paco.PacoDefs
+
+#print ITree.IEq
+#check @plfp_init
+#check @Lean.Order.lfp_monotone
+
+example {ε ρ} (t₁ t₂ : ITree ε ρ) (h : ITree.IEq t₁ t₂) : True := by
+  pinit at h
+  rw [@plfp_init (ITree ε ρ → ITree ε ρ → Lean.Order.ReverseImplicationOrder)
+    Lean.Order.instCompleteLatticePi] at h
+  trivial
